Prove theorems about stepChar. As part of that, I rewrote εClosure' to take an iterator.

RegexCorrectness/VM/CharStep/Basic.lean
@@ -4,40 +4,40 @@ set_option autoImplicit false
 
 open Regex.Data (SparseSet Vec)
 open Regex (NFA)
-open String (Pos)
+open String (Pos Iterator)
 
 namespace Regex.VM
 
 /--
-If the given state can make a transition on the given character, make the transition and traverse
-ε-closures from the resulting state. `pos` should be the position after the given character.
+If the given state can make a transition on the current character of `it`, make the transition and
+traverse ε-closures from the resulting state.
 -/
-def stepChar' (nfa : NFA) (wf : nfa.WellFormed) (c : Char) (pos : Pos)
+def stepChar' (nfa : NFA) (wf : nfa.WellFormed) (it : Iterator)
   (next : SparseSet nfa.nodes.size) (updates : Vec (List (Nat × Pos)) nfa.nodes.size)
   (state : Fin nfa.nodes.size) :
   (SparseSet nfa.nodes.size × Option (List (Nat × String.Pos)) × Vec (List (Nat × String.Pos)) nfa.nodes.size) :=
   match hn : nfa[state] with
-  | .char c' state' =>
-    if c = c' then
+  | .char c state' =>
+    if it.curr = c then
       have isLt := wf.inBounds' state hn
       let update := updates.get state state.isLt
-      εClosure' nfa wf pos next .none updates [(update, ⟨state', isLt⟩)]
+      εClosure' nfa wf it.next next .none updates [(update, ⟨state', isLt⟩)]
     else
       (next, .none, updates)
   | .sparse cs state' =>
-    if c ∈ cs then
+    if it.curr ∈ cs then
       have isLt := wf.inBounds' state hn
       let update := updates.get state state.isLt
-      εClosure' nfa wf pos next .none updates [(update, ⟨state', isLt⟩)]
+      εClosure' nfa wf it.next next .none updates [(update, ⟨state', isLt⟩)]
     else
       (next, .none, updates)
   | _ => (next, .none, updates)
 
 /--
-For all states in `current`, make a transition on the given character and traverse ε-closures from
-the resulting states.
+For all states in `current`, make a transition on the current character of `it` and traverse
+ε-closures from the resulting states.
 -/
-def eachStepChar' (nfa : NFA) (wf : nfa.WellFormed) (c : Char) (pos : Pos)
+def eachStepChar' (nfa : NFA) (wf : nfa.WellFormed) (it : Iterator)
   (current : SparseSet nfa.nodes.size) (next : SparseSet nfa.nodes.size)
   (updates : Vec (List (Nat × Pos)) nfa.nodes.size) :
   (SparseSet nfa.nodes.size × Option (List (Nat × String.Pos)) × Vec (List (Nat × String.Pos)) nfa.nodes.size) :=
@@ -49,26 +49,26 @@ where
       (next, .none, updates)
     else
       have hlt : i < current.count := Nat.lt_of_le_of_ne hle h
-      let result := stepChar' nfa wf c pos next updates current[i]
+      let result := stepChar' nfa wf it next updates current[i]
       if result.2.1.isSome then
         result
       else
         go (i + 1) hlt result.1 result.2.2
 
-theorem eachStepChar'.go.induct' (nfa : NFA) (wf : nfa.WellFormed) (c : Char) (p : Pos)
+theorem eachStepChar'.go.induct' (nfa : NFA) (wf : nfa.WellFormed) (it : Iterator)
   (current : SparseSet nfa.nodes.size)
   (motive : (i : Nat) → i ≤ current.count → SparseSet nfa.nodes.size → Vec (List (Nat × Pos)) nfa.nodes.size → Prop)
   (base : ∀ next updates, motive current.count (Nat.le_refl _) next updates)
   (found : ∀ i next updates hlt next' matched updates',
-    stepChar' nfa wf c p next updates current[i] = (next', matched, updates') →
+    stepChar' nfa wf it next updates current[i] = (next', matched, updates') →
     matched.isSome → motive i (Nat.le_of_lt hlt) next updates)
   (not_found : ∀ i next updates hlt next' matched updates',
-    stepChar' nfa wf c p next updates current[i] = (next', matched, updates') →
+    stepChar' nfa wf it next updates current[i] = (next', matched, updates') →
     ¬matched.isSome → motive (i + 1) (by omega) next' updates' →
     motive i (Nat.le_of_lt hlt) next updates)
   (i : Nat) (hle : i ≤ current.count) (next : SparseSet nfa.nodes.size) (updates : Vec (List (Nat × Pos)) nfa.nodes.size) :
   motive i hle next updates := by
-  refine eachStepChar'.go.induct nfa wf c p current motive ?base ?found ?not_found i hle next updates
+  refine eachStepChar'.go.induct nfa wf it current motive ?base ?found ?not_found i hle next updates
   case base =>
     intro next updates _
     exact base next updates
