RegexCorrectness/VM/EpsilonClosure/Lemmas.lean
@@ -1,5 +1,6 @@
 import RegexCorrectness.Data.SparseSet
 import RegexCorrectness.NFA.Semantics.Path
+import RegexCorrectness.VM.Basic2
 import RegexCorrectness.VM.EpsilonClosure.Basic
 import RegexCorrectness.VM.EpsilonClosure.Path
 
@@ -8,19 +9,19 @@ set_option autoImplicit false
 open Regex.Data (SparseSet Vec Span)
 open Regex (NFA)
 open Regex.NFA (εStep' εClosure')
-open String (Pos)
+open String (Pos Iterator)
 
 namespace Regex.VM
 
-variable {nfa : NFA} {wf : nfa.WellFormed} {pos : Pos}
+variable {nfa : NFA} {wf : nfa.WellFormed} {it : Iterator}
   {next : SparseSet nfa.nodes.size} {matched : Option (List (Nat × Pos))}
   {updates : Vec (List (Nat × String.Pos)) nfa.nodes.size} {stack : εStack' nfa}
   {next' : SparseSet nfa.nodes.size} {matched' : Option (List (Nat × Pos))}
   {updates' : Vec (List (Nat × String.Pos)) nfa.nodes.size}
 
-theorem εClosure.subset (h : εClosure' nfa wf pos next matched updates stack = (next', matched', updates')) :
+theorem εClosure.subset (h : εClosure' nfa wf it next matched updates stack = (next', matched', updates')) :
   next ⊆ next' := by
-  induction next, matched, updates, stack using εClosure'.induct' nfa wf pos with
+  induction next, matched, updates, stack using εClosure'.induct' nfa wf it with
   | base next matched updates =>
     simp [εClosure'_base] at h
     simp [h]
@@ -50,10 +51,10 @@ theorem εClosure.subset (h : εClosure' nfa wf pos next matched updates stack =
     rw [εClosure'_fail mem hn] at h
     exact (SparseSet.subset_trans SparseSet.subset_insert (ih h))
 
-theorem εClosure.mem_next_of_mem_stack {i update} (h : εClosure' nfa wf pos next matched updates stack = (next', matched', updates'))
+theorem εClosure.mem_next_of_mem_stack {i update} (h : εClosure' nfa wf it next matched updates stack = (next', matched', updates'))
   (mem_stack : (update, i) ∈ stack) :
   i ∈ next' := by
-  induction next, matched, updates, stack using εClosure'.induct' nfa wf pos with
+  induction next, matched, updates, stack using εClosure'.induct' nfa wf it with
   | base next matched updates => simp at mem_stack
   | visited next matched updates update state stack mem ih =>
     rw [εClosure'_visited mem] at h
@@ -138,10 +139,10 @@ theorem εClosure.LowerBound.of_step (h : εClosure.LowerBoundStep next) : εClo
   | base => exact mem
   | step step _ ih => exact ih (h _ _ _ _ mem step)
 
-theorem εClosure.lower_bound_step (h : εClosure' nfa wf pos next matched updates stack = (next', matched', updates'))
+theorem εClosure.lower_bound_step (h : εClosure' nfa wf it next matched updates stack = (next', matched', updates'))
   (inv : εClosure.LowerInvStep next stack) :
   εClosure.LowerBoundStep next' := by
-  induction next, matched, updates, stack using εClosure'.induct' nfa wf pos with
+  induction next, matched, updates, stack using εClosure'.induct' nfa wf it with
   | base next matched updates =>
     simp_all
     intro i j span update mem step
@@ -199,12 +200,12 @@ theorem εClosure.lower_bound_step (h : εClosure' nfa wf pos next matched updat
     exact ih h inv'
   | save next matched updates update state stack' offset state' mem hn ih =>
     rw [εClosure'_save mem hn] at h
-    have inv' : εClosure.LowerInvStep (next.insert state) ((update ++ [(offset, pos)], state') :: stack') := by
+    have inv' : εClosure.LowerInvStep (next.insert state) ((update ++ [(offset, it.pos)], state') :: stack') := by
       intro i j span update' mem' step'
       cases SparseSet.eq_or_mem_of_mem_insert mem' with
       | inl eq =>
         simp [eq, εStep'.save hn] at step'
-        exact .inr ⟨update ++ [(offset, pos)], by simp [step']⟩
+        exact .inr ⟨update ++ [(offset, it.pos)], by simp [step']⟩
       | inr mem'' =>
         match inv i j span update' mem'' step' with
         | .inl mem => exact .inl (SparseSet.mem_insert_of_mem mem)
@@ -275,7 +276,7 @@ theorem εClosure.lower_bound_step (h : εClosure' nfa wf pos next matched updat
           | inr mem => exact .inr ⟨update'', by simp [mem]⟩
     exact ih h inv'
 
-theorem εClosure.lower_bound {i update} (h : εClosure' nfa wf pos next matched updates [(update, i)] = (next', matched', updates'))
+theorem εClosure.lower_bound {i update} (h : εClosure' nfa wf it next matched updates [(update, i)] = (next', matched', updates'))
   (lb : εClosure.LowerBound next) :
   εClosure.LowerBound next' := by
   have inv : εClosure.LowerInvStep next [(update, i)] := by
@@ -284,49 +285,43 @@ theorem εClosure.lower_bound {i update} (h : εClosure' nfa wf pos next matched
   have lb_step := εClosure.lower_bound_step h inv
   exact εClosure.LowerBound.of_step lb_step
 
--- TODO: move this to a shared file
 /--
-As an optimization, we write the updates to the buffer only when the state is done, a character, or a sparse state.
--/
-def WriteUpdate (i : Fin nfa.nodes.size) : Prop :=
-  match nfa[i] with
-  | .done | .char _ _ | .sparse _ _ => True
-  | _ => False
+Intuition: given that we reached `i₀` (from `nfa.start`) with `span₀` and `update₀`, the εClosure
+traversal first puts states reachable from `i₀` into the stack with an appropriate update list.
+Next, the traversal pops the states from the stack and writes them to `next`, recording the update
+list to `updates` for the necessary states. Since we only care about ε-transitions, span doesn't
+change during the traversal.
 
-/--
-Intuition: given the starting state `i₀` and the updates `update₀` at `i₀`, the εClosure traversal
-first puts states reachable from `i₀` into the stack with an appropriate update list. Next, the
-traversal pops the states from the stack and writes them to `next`, recording the update list to
-`updates` for the necessary states.
-
-Therefore, at the end of the traversal, we can guarantee that all states in `next` were already in `next₀`
-or they are reachable from `i₀` with the updates written to `updates`.
+At the end of the traversal, we can guarantee that all states in `next` were already in `next₀` or
+they are reachable from `i₀` with the updates written to `updates`.
 -/
-structure εClosure.UpperInv (pos : Pos) (next₀ : SparseSet nfa.nodes.size) (i₀ : Fin nfa.nodes.size) (update₀ : List (Nat × Pos))
+structure εClosure.UpperInv (next₀ : SparseSet nfa.nodes.size) (span₀ : Span) (i₀ : Fin nfa.nodes.size) (update₀ : List (Nat × Pos))
   (next : SparseSet nfa.nodes.size) (updates : Vec (List (Nat × Pos)) nfa.nodes.size) (stack : εStack' nfa) : Prop where
   -- The intuition is that `update₀` corresponds to the update list from `nfa.start` to `i₀`, and
   -- `update'` is the update list from `i₀` to `j`. Therefore, `update₀ ++ update'` gives the update
   -- list from `nfa.start` to `j`.
-  mem_stack : ∀ update j, (update, j) ∈ stack → ∃ span update', span.curr = pos ∧ update = update₀ ++ update' ∧ nfa.εClosure' span i₀ j update'
-  mem_next : ∀ j ∈ next, j ∈ next₀ ∨
-    ∃ span update', span.curr = pos ∧ nfa.εClosure' span i₀ j update' ∧ (WriteUpdate j → updates[j] = update₀ ++ update')
+  mem_stack : ∀ update j, (update, j) ∈ stack →
+    ∃ update', update = update₀ ++ update' ∧ nfa.εClosure' span₀ i₀ j update'
+  mem_next : ∀ j ∈ next,
+    j ∈ next₀ ∨ ∃ update', nfa.εClosure' span₀ i₀ j update' ∧ (WriteUpdate j → updates[j] = update₀ ++ update')
 
 /--
 All new states in `next'` are reachable from the starting state `i₀` and have corresponding updates in `updates'`.
 -/
-theorem εClosure.upper_boundAux (next₀ : SparseSet nfa.nodes.size) (i₀ : Fin nfa.nodes.size) (update₀ : List (Nat × Pos))
-  (h : εClosure' nfa wf pos next matched updates stack = (next', matched', updates'))
-  (inv₀ : εClosure.UpperInv pos next₀ i₀ update₀ next updates stack) :
-  εClosure.UpperInv pos next₀ i₀ update₀ next' updates' []  := by
-  induction next, matched, updates, stack using εClosure'.induct' nfa wf pos with
+theorem εClosure.upper_boundAux (next₀ : SparseSet nfa.nodes.size) (span₀ : Span) (i₀ : Fin nfa.nodes.size) (update₀ : List (Nat × Pos))
+  (eq_curr : span₀.curr = it.pos)
+  (h : εClosure' nfa wf it next matched updates stack = (next', matched', updates'))
+  (inv₀ : εClosure.UpperInv next₀ span₀ i₀ update₀ next updates stack) :
+  εClosure.UpperInv next₀ span₀ i₀ update₀ next' updates' []  := by
+  induction next, matched, updates, stack using εClosure'.induct' nfa wf it with
   | base next matched updates =>
     simp [εClosure'_base] at h
     simp [h] at inv₀
     exact inv₀
   | visited next matched updates update state stack mem ih =>
     rw [εClosure'_visited mem] at h
-    have inv' : εClosure.UpperInv pos next₀ i₀ update₀ next updates stack := by
-      have ⟨span, update', eqp, equ, cls⟩ := inv₀.mem_stack update state (by simp)
+    have inv' : εClosure.UpperInv next₀ span₀ i₀ update₀ next updates stack := by
+      have ⟨update', equ, cls⟩ := inv₀.mem_stack update state (by simp)
       refine ⟨?mem_stack, ?mem_next⟩
       case mem_stack =>
         intro u j mem
@@ -337,8 +332,8 @@ theorem εClosure.upper_boundAux (next₀ : SparseSet nfa.nodes.size) (i₀ : Fi
     exact ih h inv'
   | epsilon next matched updates update state stack' state' mem hn ih =>
     rw [εClosure'_epsilon mem hn] at h
-    have inv' : εClosure.UpperInv pos next₀ i₀ update₀ (next.insert state) updates ((update, state') :: stack') := by
-      have ⟨span, update', eqp, equ, cls⟩ := inv₀.mem_stack update state (by simp)
+    have inv' : εClosure.UpperInv next₀ span₀ i₀ update₀ (next.insert state) updates ((update, state') :: stack') := by
+      have ⟨update', equ, cls⟩ := inv₀.mem_stack update state (by simp)
       refine ⟨?mem_stack, ?mem_next⟩
       case mem_stack =>
         intro u j mem
@@ -346,24 +341,24 @@ theorem εClosure.upper_boundAux (next₀ : SparseSet nfa.nodes.size) (i₀ : Fi
         match mem with
         | .inl ⟨equ, eqj⟩ =>
           subst u j
-          have step : nfa.εStep' span state state' .none := by
+          have step : nfa.εStep' span₀ state state' .none := by
             simp [εStep'.epsilon hn]
           have cls' := cls.snoc step
           simp at cls'
-          exact ⟨span, update', eqp, equ, cls'⟩
+          exact ⟨update', equ, cls'⟩
         | .inr mem => exact inv₀.mem_stack u j (by simp [mem])
       case mem_next =>
         intro j mem
         cases SparseSet.eq_or_mem_of_mem_insert mem with
         | inl eq =>
           subst j
-          exact .inr ⟨span, update', eqp, cls, by simp [WriteUpdate, hn]⟩
+          exact .inr ⟨update', cls, by simp [WriteUpdate, hn]⟩
         | inr mem => exact inv₀.mem_next j mem
     exact ih h inv'
   | split next matched updates update state stack' state₁ state₂ mem hn ih =>
     rw [εClosure'_split mem hn] at h
-    have inv' : εClosure.UpperInv pos next₀ i₀ update₀ (next.insert state) updates ((update, state₁) :: (update, state₂) :: stack') := by
-      have ⟨span, update', eqp, equ, cls⟩ := inv₀.mem_stack update state (by simp)
+    have inv' : εClosure.UpperInv next₀ span₀ i₀ update₀ (next.insert state) updates ((update, state₁) :: (update, state₂) :: stack') := by
+      have ⟨update', equ, cls⟩ := inv₀.mem_stack update state (by simp)
       refine ⟨?mem_stack, ?mem_next⟩
       case mem_stack =>
         intro u j mem
@@ -371,31 +366,31 @@ theorem εClosure.upper_boundAux (next₀ : SparseSet nfa.nodes.size) (i₀ : Fi
         match mem with
         | .inl ⟨equ, eqj⟩ =>
           subst u j
-          have step : nfa.εStep' span state state₁ .none := by
+          have step : nfa.εStep' span₀ state state₁ .none := by
             simp [εStep'.split hn]
           have cls' := cls.snoc step
           simp at cls'
-          exact ⟨span, update', eqp, equ, cls'⟩
+          exact ⟨update', equ, cls'⟩
         | .inr (.inl ⟨equ, eqj⟩) =>
           subst u j
-          have step : nfa.εStep' span state state₂ .none := by
+          have step : nfa.εStep' span₀ state state₂ .none := by
             simp [εStep'.split hn]
           have cls' := cls.snoc step
           simp at cls'
-          exact ⟨span, update', eqp, equ, cls'⟩
+          exact ⟨update', equ, cls'⟩
         | .inr (.inr mem) => exact inv₀.mem_stack u j (by simp [mem])
       case mem_next =>
         intro j mem
         cases SparseSet.eq_or_mem_of_mem_insert mem with
         | inl eq =>
           subst j
-          exact .inr ⟨span, update', eqp, cls, by simp [WriteUpdate, hn]⟩
+          exact .inr ⟨update', cls, by simp [WriteUpdate, hn]⟩
         | inr mem => exact inv₀.mem_next j mem
     exact ih h inv'
   | save next matched updates update state stack' offset state' mem hn ih =>
     rw [εClosure'_save mem hn] at h
-    have inv' : εClosure.UpperInv pos next₀ i₀ update₀ (next.insert state) updates ((update ++ [(offset, pos)], state') :: stack') := by
-      have ⟨span, update', eqp, equ, cls⟩ := inv₀.mem_stack update state (by simp)
+    have inv' : εClosure.UpperInv next₀ span₀ i₀ update₀ (next.insert state) updates ((update ++ [(offset, it.pos)], state') :: stack') := by
+      have ⟨update', equ, cls⟩ := inv₀.mem_stack update state (by simp)
       refine ⟨?mem_stack, ?mem_next⟩
       case mem_stack =>
         intro u j mem
@@ -403,18 +398,17 @@ theorem εClosure.upper_boundAux (next₀ : SparseSet nfa.nodes.size) (i₀ : Fi
         match mem with
         | .inl ⟨equ', eqj⟩ =>
           subst u j
-          have last : nfa.εStep' span state state' (.some (offset, span.curr)) :=
+          have last : nfa.εStep' span₀ state state' (.some (offset, span₀.curr)) :=
             NFA.Step.save (Nat.zero_le _) state.isLt hn
-          have := eqp ▸ cls.snoc last
-          simp at this
-          exact ⟨span, update' ++ [(offset, pos)], eqp, by simp [equ], this⟩
+          have := cls.snoc last
+          exact ⟨update' ++ [(offset, it.pos)], by simp [equ], eq_curr ▸ this⟩
         | .inr mem => exact inv₀.mem_stack u j (by simp [mem])
       case mem_next =>
         intro j mem
         cases SparseSet.eq_or_mem_of_mem_insert mem with
         | inl eq =>
           subst j
-          exact .inr ⟨span, update', eqp, cls, by simp [WriteUpdate, hn]⟩
+          exact .inr ⟨update', cls, by simp [WriteUpdate, hn]⟩
         | inr mem => exact inv₀.mem_next j mem
     exact ih h inv'
   | done next matched updates update state stack' mem hn ih =>
@@ -428,8 +422,8 @@ theorem εClosure.upper_boundAux (next₀ : SparseSet nfa.nodes.size) (i₀ : Fi
     exact ih h (inv_done_char_sparse inv₀)
   | fail next matched updates update state stack' mem hn ih =>
     rw [εClosure'_fail mem hn] at h
-    have inv' : εClosure.UpperInv pos next₀ i₀ update₀ (next.insert state) updates stack' := by
-      have ⟨span, update', eqp, equ, cls⟩ := inv₀.mem_stack update state (by simp)
+    have inv' : εClosure.UpperInv next₀ span₀ i₀ update₀ (next.insert state) updates stack' := by
+      have ⟨update', equ, cls⟩ := inv₀.mem_stack update state (by simp)
       refine ⟨?mem_stack, ?mem_next⟩
       case mem_stack =>
         intro u j mem
@@ -439,14 +433,14 @@ theorem εClosure.upper_boundAux (next₀ : SparseSet nfa.nodes.size) (i₀ : Fi
         cases SparseSet.eq_or_mem_of_mem_insert mem with
         | inl eq =>
           subst j
-          exact .inr ⟨span, update', eqp, cls, by simp [WriteUpdate, hn]⟩
+          exact .inr ⟨update', cls, by simp [WriteUpdate, hn]⟩
         | inr mem => exact inv₀.mem_next j mem
     exact ih h inv'
 where
   inv_done_char_sparse {next updates state update stack'}
-    (inv₀ : εClosure.UpperInv pos next₀ i₀ update₀ next updates ((update, state) :: stack')) :
-    εClosure.UpperInv pos next₀ i₀ update₀ (next.insert state) (updates.set state state.isLt update) stack' := by
-    have ⟨span, update', eqp, equ, cls⟩ := inv₀.mem_stack update state (by simp)
+    (inv₀ : εClosure.UpperInv next₀ span₀ i₀ update₀ next updates ((update, state) :: stack')) :
+    εClosure.UpperInv next₀ span₀ i₀ update₀ (next.insert state) (updates.set state state.isLt update) stack' := by
+    have ⟨update', equ, cls⟩ := inv₀.mem_stack update state (by simp)
     refine ⟨?mem_stack, ?mem_next⟩
     case mem_stack =>
       intro u j mem
@@ -456,46 +450,46 @@ where
       cases SparseSet.eq_or_mem_of_mem_insert mem with
       | inl eq =>
         subst j
-        exact .inr ⟨span, update', eqp, cls, by simp [equ]⟩
+        exact .inr ⟨update', cls, by simp [equ]⟩
       | inr mem =>
         match inv₀.mem_next j mem with
         | .inl mem => exact .inl mem
-        | .inr ⟨span', update'', cls', h⟩ =>
+        | .inr ⟨update'', cls', h⟩ =>
           if h' : state = j then
             subst j
-            exact .inr ⟨span, update', eqp, cls, by simp [equ]⟩
+            exact .inr ⟨update', cls, by simp [equ]⟩
           else
             have : state.val ≠ j.val := by omega
-            exact .inr ⟨span', update'', cls', by simp [this]; exact h⟩
+            exact .inr ⟨update'', cls', by simp [this]; exact h⟩
 
 /--
 Upper invariant at the start of the εClosure traversal. The caller needs to supply a span that
 corresponds to the given `pos`.
 -/
-theorem εClosure.UpperInv.intro {next₀ i₀ update₀} (span₀ : Span) (hspan₀ : span₀.curr = pos) :
-  εClosure.UpperInv pos next₀ i₀ update₀ next₀ updates [(update₀, i₀)] := by
+theorem εClosure.UpperInv.intro {next₀ i₀ update₀} (span₀ : Span) :
+  εClosure.UpperInv next₀ span₀ i₀ update₀ next₀ updates [(update₀, i₀)] := by
   refine ⟨?mem_stack, ?mem_next⟩
   case mem_stack =>
     intro update j mem
     simp at mem
     simp [mem]
-    exact ⟨span₀, hspan₀, .base⟩
+    exact .base
   case mem_next =>
     intro j mem
     exact .inl mem
 
-theorem εClosure.upper_bound {i update} (span₀ : Span) (hspan₀ : span₀.curr = pos)
-  (h : εClosure' nfa wf pos next matched updates [(update, i)] = (next', matched', updates')) :
+theorem εClosure.upper_bound {i update} (span : Span) (eq_curr : span.curr = it.pos)
+  (h : εClosure' nfa wf it next matched updates [(update, i)] = (next', matched', updates')) :
   ∀ j ∈ next', j ∈ next ∨
-    ∃ span update', span.curr = pos ∧ nfa.εClosure' span i j update' ∧ (WriteUpdate j → updates'[j] = update ++ update') := by
-  have := εClosure.upper_boundAux next i update h (εClosure.UpperInv.intro span₀ hspan₀)
+    ∃ update', nfa.εClosure' span i j update' ∧ (WriteUpdate j → updates'[j] = update ++ update') := by
+  have := εClosure.upper_boundAux next span i update eq_curr h (εClosure.UpperInv.intro span)
   exact this.mem_next
 
 /--
 `εClosure'` inserts all states in the ε-closure of `i` into `next`.
 -/
 theorem mem_next_of_εClosure {i update}
-  (h : εClosure' nfa wf pos next matched updates [(update, i)] = (next', matched', updates'))
+  (h : εClosure' nfa wf it next matched updates [(update, i)] = (next', matched', updates'))
   (lb : εClosure.LowerBound next)
   {j span update'} (cls : nfa.εClosure' span i j update') :
   j ∈ next' := by
@@ -503,15 +497,23 @@ theorem mem_next_of_εClosure {i update}
   exact εClosure.lower_bound h lb _ _ _ _ this cls
 
 /--
+All states in `next'` are already in `next` or they are reachable from `i` with the updates written to `updates`.
+-/
+theorem write_updates_of_mem_next_of_εClosure {i j update} (span : Span) (eq_curr : span.curr = it.pos)
+  (h : εClosure' nfa wf it next matched updates [(update, i)] = (next', matched', updates'))
+  (mem : j ∈ next') :
+  j ∈ next ∨ ∃ update', nfa.εClosure' span i j update' ∧ (WriteUpdate j → updates'[j] = update ++ update') :=
+  εClosure.upper_bound span eq_curr h j mem
+
+/--
 For all states in the ε-closure of `i`, it's already in `next` or there is a path from `i` whose
 updates are written to `updates`. The written update list can be different since the traversal
 may have reached the state through a different path.
 -/
-theorem write_updates_of_εClosure {i update} (span₀ : Span) (hspan₀ : span₀.curr = pos)
-  (h : εClosure' nfa wf pos next matched updates [(update, i)] = (next', matched', updates'))
-  (lb : εClosure.LowerBound next)
-  {j span update'} (cls : nfa.εClosure' span i j update') :
-  j ∈ next ∨ ∃ span update', span.curr = pos ∧ nfa.εClosure' span i j update' ∧ (WriteUpdate j → updates'[j] = update ++ update') :=
-  εClosure.upper_bound span₀ hspan₀ h _ (mem_next_of_εClosure h lb cls)
+theorem write_updates_of_εClosure {i j update update'} (span : Span) (eq_curr : span.curr = it.pos)
+  (h : εClosure' nfa wf it next matched updates [(update, i)] = (next', matched', updates'))
+  (lb : εClosure.LowerBound next) (cls : nfa.εClosure' span i j update') :
+  j ∈ next ∨ ∃ update', nfa.εClosure' span i j update' ∧ (WriteUpdate j → updates'[j] = update ++ update') :=
+  write_updates_of_mem_next_of_εClosure span eq_curr h (mem_next_of_εClosure h lb cls)
 
 end Regex.VM
