RegexCorrectness/VM/Basic2.lean
@@ -1,0 +1,13 @@
+import Regex.NFA
+
+namespace Regex.VM
+
+/--
+As an optimization, we write the updates to the buffer only when the state is done, a character, or a sparse state.
+-/
+def WriteUpdate {nfa : NFA} (i : Fin nfa.nodes.size) : Prop :=
+  match nfa[i] with
+  | .done | .char _ _ | .sparse _ _ => True
+  | _ => False
+
+end Regex.VM
