RegexCorrectness/VM/CharStep/Lemmas.lean
@@ -1,0 +1,90 @@
+import RegexCorrectness.VM.EpsilonClosure
+import RegexCorrectness.VM.CharStep.Basic
+import RegexCorrectness.VM.CharStep.Path
+
+set_option autoImplicit false
+
+open Regex.Data (SparseSet Vec Span)
+open Regex (NFA)
+open Regex.NFA (εStep' εClosure' CharStep)
+open String (Pos Iterator)
+
+namespace Regex.VM
+
+variable {nfa : NFA} {wf : nfa.WellFormed} {it : Iterator}
+  {current next : SparseSet nfa.nodes.size} {updates : Vec (List (Nat × String.Pos)) nfa.nodes.size}
+  {state : Fin nfa.nodes.size}
+  {next' : SparseSet nfa.nodes.size} {matched' : Option (List (Nat × Pos))}
+  {updates' : Vec (List (Nat × String.Pos)) nfa.nodes.size}
+
+theorem stepChar.lower_bound (h : stepChar' nfa wf it next updates state = (next', matched', updates'))
+  (lb : εClosure.LowerBound next) :
+  εClosure.LowerBound next' := by
+  simp [stepChar'] at h
+  split at h
+  next c' state' hn =>
+    split at h
+    next eq => exact εClosure.lower_bound h lb
+    next => simp_all
+  next cs state' =>
+    split at h
+    next eq => exact εClosure.lower_bound h lb
+    next => simp_all
+  next => simp_all
+
+theorem mem_next_of_stepChar {l m r i j k update}
+  (h : stepChar' nfa wf it next updates i = (next', matched', updates'))
+  (lb : εClosure.LowerBound next)
+  (step : nfa.CharStep l m it.curr r i j) (cls : nfa.εClosure' ⟨l, it.curr :: m, r⟩ j k update) :
+  k ∈ next' := by
+  simp [stepChar'] at h
+  split at h
+  next c' j' hn =>
+    rw [CharStep.char hn] at step
+    simp [←step] at h
+    apply mem_next_of_εClosure h lb cls
+  next cs j' hn =>
+    rw [CharStep.sparse hn] at step
+    simp [step.1, ←step.2] at h
+    apply mem_next_of_εClosure h lb cls
+  next ne₁ ne₂ =>
+    have := step.char_or_sparse
+    simp_all
+
+theorem write_updates_of_mem_next_of_stepChar {i k} (span : Span) (hspan : span.iterator = it)
+  (h : stepChar' nfa wf it next updates i = (next', matched', updates'))
+  (notEnd : ¬it.atEnd) (mem : k ∈ next') :
+  k ∈ next ∨ ∃ r' j update',
+    span.r = it.curr :: r' ∧
+    nfa.CharStep span.l span.m it.curr r' i j ∧
+    nfa.εClosure' span.next j k update' ∧
+    (WriteUpdate k → updates'[k] = updates.get i i.isLt ++ update') := by
+  simp [stepChar'] at h
+  split at h
+  next c j hn =>
+    split at h
+    next eqc =>
+      subst it c
+      have ⟨r', eqr⟩ := span.exists_cons_of_not_atEnd notEnd
+      have := write_updates_of_mem_next_of_εClosure span.next (span.next_curr_eq_next_pos eqr) h mem
+      match this with
+      | .inl mem => exact .inl mem
+      | .inr ⟨update', cls, write⟩ =>
+        have isLt := wf.inBounds' i hn
+        exact .inr ⟨r', ⟨j, isLt⟩, update', eqr, NFA.Step.char (Nat.zero_le _) i.isLt hn, cls, write⟩
+    next => simp_all only [SparseSet.mem_mem, Prod.mk.injEq, exists_and_left, true_or]
+  next cs j hn =>
+    split at h
+    next cmem =>
+      subst it
+      have ⟨r', eqr⟩ := span.exists_cons_of_not_atEnd notEnd
+      have := write_updates_of_mem_next_of_εClosure span.next (span.next_curr_eq_next_pos eqr) h mem
+      match this with
+      | .inl mem => exact .inl mem
+      | .inr ⟨update', cls, write⟩ =>
+        have isLt := wf.inBounds' i hn
+        exact .inr ⟨r', ⟨j, isLt⟩, update', eqr, NFA.Step.sparse (Nat.zero_le _) i.isLt hn cmem, cls, write⟩
+    next => simp_all only [SparseSet.mem_mem, Prod.mk.injEq, exists_and_left, true_or]
+  next => simp_all only [SparseSet.mem_mem, Prod.mk.injEq, exists_and_left, true_or]
+
+end Regex.VM
