RegexCorrectness/VM/CharStep/Path.lean
@@ -1,0 +1,69 @@
+import RegexCorrectness.NFA.Semantics.Path
+
+set_option autoImplicit false
+
+open Regex.Data (Span)
+
+namespace Regex.NFA
+
+def CharStep (nfa : NFA) (l m : List Char) (c : Char) (r : List Char) (i j : Fin nfa.nodes.size) : Prop :=
+  nfa.Step 0 i ⟨l, m, c :: r⟩ j ⟨l, c :: m, r⟩ .none
+
+namespace CharStep
+
+variable {nfa : NFA} {l m : List Char} {c : Char} {r : List Char} {i j : Fin nfa.nodes.size}
+
+@[simp]
+theorem done (hn : nfa[i] = .done) :
+  nfa.CharStep l m c r i j ↔ False := by
+  apply Step.iff_done hn
+
+@[simp]
+theorem fail (hn : nfa[i] = .fail) :
+  nfa.CharStep l m c r i j ↔ False := by
+  apply Step.iff_fail hn
+
+@[simp]
+theorem epsilon {next} (hn : nfa[i] = .epsilon next) :
+  nfa.CharStep l m c r i j ↔ False := by
+  simp [CharStep, Step.iff_epsilon hn]
+
+@[simp]
+theorem split {next₁ next₂} (hn : nfa[i] = .split next₁ next₂) :
+  nfa.CharStep l m c r i j ↔ False := by
+  simp [CharStep, Step.iff_split hn]
+
+@[simp]
+theorem save {offset next} (hn : nfa[i] = .save offset next) :
+  nfa.CharStep l m c r i j ↔ False := by
+  simp [CharStep, Step.iff_save hn]
+
+@[simp]
+theorem char {c' next} (hn : nfa[i] = .char c' next) :
+  nfa.CharStep l m c r i j ↔ c = c' ∧ j = next := by
+  simp [CharStep, Step.iff_char]
+  apply Iff.intro
+  . intro step
+    cases step <;> simp_all
+  . intro eq
+    simp [eq]
+    exact Step.char (Nat.zero_le _) i.isLt hn
+
+@[simp]
+theorem sparse {cs next} (hn : nfa[i] = .sparse cs next) :
+  nfa.CharStep l m c r i j ↔ c ∈ cs ∧ j = next := by
+  rw [CharStep]
+  apply Iff.intro
+  . intro step
+    cases step <;> simp_all
+  . intro ⟨mem, eq⟩
+    simp [eq]
+    exact Step.sparse (Nat.zero_le _) i.isLt hn mem
+
+theorem char_or_sparse (step : nfa.CharStep l m c r i j) :
+  (∃ c' next, nfa[i] = .char c' next) ∨ (∃ cs next, nfa[i] = .sparse cs next) := by
+  cases step <;> simp_all
+
+end CharStep
+
+end Regex.NFA
