RegexCorrectness/VM/EpsilonClosure/Basic.lean
@@ -7,56 +7,56 @@ set_option autoImplicit false
 
 open Regex.Data (SparseSet Vec)
 open Regex (NFA)
-open String (Pos)
+open String (Pos Iterator)
 
 namespace Regex.VM
 
-abbrev εStack' (nfa : NFA) := List (List (Nat × String.Pos) × Fin nfa.nodes.size)
+abbrev εStack' (nfa : NFA) := List (List (Nat × Pos) × Fin nfa.nodes.size)
 
 /--
 A version of εClosure traversal that tracks the updates to the capture groups.
 
-As the NFA semantics use `List (Nat × String.Pos)` to represent the capture group updates, this
+As the NFA semantics use `List (Nat × Pos)` to represent the capture group updates, this
 εClosure implementation also use it for verification. The actual VM implementation materializes the
 updates as a `Buffer` for efficiency, and the correspondence will be proved in `Correspondence.lean`.
 -/
-def εClosure' (nfa : NFA) (wf : nfa.WellFormed) (pos : Pos)
-  (next : SparseSet nfa.nodes.size) (matched : Option (List (Nat × String.Pos))) (updates : Vec (List (Nat × String.Pos)) nfa.nodes.size)
+def εClosure' (nfa : NFA) (wf : nfa.WellFormed) (it : Iterator)
+  (next : SparseSet nfa.nodes.size) (matched : Option (List (Nat × Pos))) (updates : Vec (List (Nat × Pos)) nfa.nodes.size)
   (stack : εStack' nfa) :
-  (SparseSet nfa.nodes.size × Option (List (Nat × String.Pos)) × Vec (List (Nat × String.Pos)) nfa.nodes.size) :=
+  (SparseSet nfa.nodes.size × Option (List (Nat × Pos)) × Vec (List (Nat × Pos)) nfa.nodes.size) :=
   match stack with
   | [] => (next, matched, updates)
   | (update, state) :: stack' =>
     if state ∈ next then
-      εClosure' nfa wf pos next matched updates stack'
+      εClosure' nfa wf it next matched updates stack'
     else
       let next' := next.insert state
       match hn : nfa[state] with
       | .epsilon state' =>
         have isLt : state' < nfa.nodes.size := wf.inBounds' state hn
-        εClosure' nfa wf pos next' matched updates ((update, ⟨state', isLt⟩) :: stack')
+        εClosure' nfa wf it next' matched updates ((update, ⟨state', isLt⟩) :: stack')
       | .split state₁ state₂ =>
         have isLt : state₁ < nfa.nodes.size ∧ state₂ < nfa.nodes.size := wf.inBounds' state hn
-        εClosure' nfa wf pos next' matched updates ((update, ⟨state₁, isLt.1⟩) :: (update, ⟨state₂, isLt.2⟩):: stack')
+        εClosure' nfa wf it next' matched updates ((update, ⟨state₁, isLt.1⟩) :: (update, ⟨state₂, isLt.2⟩):: stack')
       | .save offset state' =>
         have isLt : state' < nfa.nodes.size := wf.inBounds' state hn
-        let update' := update ++ [(offset, pos)]
-        εClosure' nfa wf pos next' matched updates ((update', ⟨state', isLt⟩) :: stack')
+        let update' := update ++ [(offset, it.pos)]
+        εClosure' nfa wf it next' matched updates ((update', ⟨state', isLt⟩) :: stack')
       | .done =>
         let matched' := matched <|> update
         let buffers' := updates.set state state.isLt update
-        εClosure' nfa wf pos next' matched' buffers' stack'
+        εClosure' nfa wf it next' matched' buffers' stack'
       | .char c state' =>
         let buffers' := updates.set state state.isLt update
-        εClosure' nfa wf pos next' matched buffers' stack'
+        εClosure' nfa wf it next' matched buffers' stack'
       | .sparse cs state' =>
         let buffers' := updates.set state state.isLt update
-        εClosure' nfa wf pos next' matched buffers' stack'
-      | .fail => εClosure' nfa wf pos next' matched updates stack'
+        εClosure' nfa wf it next' matched buffers' stack'
+      | .fail => εClosure' nfa wf it next' matched updates stack'
 termination_by (next.measure, stack)
 
 -- Tidied up version of the function induction
-theorem εClosure'.induct' (nfa : NFA) (wf : nfa.WellFormed) (pos : Pos)
+theorem εClosure'.induct' (nfa : NFA) (wf : nfa.WellFormed) (it : Iterator)
   (motive : SparseSet nfa.nodes.size → Option (List (Nat × Pos)) → Vec (List (Nat × Pos)) nfa.nodes.size → εStack' nfa → Prop)
   (base : ∀ next matched updates, motive next matched updates [])
   (visited : ∀ next matched updates update state stack',
@@ -72,7 +72,7 @@ theorem εClosure'.induct' (nfa : NFA) (wf : nfa.WellFormed) (pos : Pos)
     motive next matched updates ((update, state) :: stack'))
   (save : ∀ next matched updates update state stack' offset state',
     state ∉ next → nfa[state] = .save offset state' →
-    motive (next.insert state) matched updates ((update ++ [(offset, pos)], state') :: stack') →
+    motive (next.insert state) matched updates ((update ++ [(offset, it.pos)], state') :: stack') →
     motive next matched updates ((update, state) :: stack'))
   (done : ∀ next matched updates update state stack',
     state ∉ next → nfa[state] = .done →
@@ -91,7 +91,7 @@ theorem εClosure'.induct' (nfa : NFA) (wf : nfa.WellFormed) (pos : Pos)
     motive (next.insert state) matched updates stack' →
     motive next matched updates ((update, state) :: stack')) :
   ∀ next matched updates stack, motive next matched updates stack := by
-  refine εClosure'.induct nfa wf pos motive base visited ?epsilon ?split ?save ?done ?char ?sparse ?fail
+  refine εClosure'.induct nfa wf it motive base visited ?epsilon ?split ?save ?done ?char ?sparse ?fail
   case epsilon =>
     intro next matched updates update state stack' hmem next' state' hn isLt ih
     exact epsilon next matched updates update state stack' ⟨state', isLt⟩ hmem hn ih
@@ -119,20 +119,20 @@ Simplification lemmas for `εClosure'`.
 -/
 section
 
-variable {nfa wf pos next matched updates}
+variable {nfa wf it next matched updates}
 
 @[simp]
-theorem εClosure'_base : εClosure' nfa wf pos next matched updates [] = (next, matched, updates) := by
+theorem εClosure'_base : εClosure' nfa wf it next matched updates [] = (next, matched, updates) := by
   simp [εClosure']
 
 @[simp]
 theorem εClosure'_visited {update state stack'} (hmem : state ∈ next) :
-  εClosure' nfa wf pos next matched updates ((update, state) :: stack') = εClosure' nfa wf pos next matched updates stack' := by
+  εClosure' nfa wf it next matched updates ((update, state) :: stack') = εClosure' nfa wf it next matched updates stack' := by
   simp [εClosure', hmem]
 
 @[simp]
 theorem εClosure'_epsilon {update state stack' state'} (hmem : state ∉ next) (hn : nfa[state] = .epsilon state') :
-  εClosure' nfa wf pos next matched updates ((update, state) :: stack') = εClosure' nfa wf pos (next.insert state) matched updates ((update, state') :: stack') := by
+  εClosure' nfa wf it next matched updates ((update, state) :: stack') = εClosure' nfa wf it (next.insert state) matched updates ((update, state') :: stack') := by
   conv =>
     lhs
     unfold εClosure'
@@ -141,7 +141,7 @@ theorem εClosure'_epsilon {update state stack' state'} (hmem : state ∉ next) 
 
 @[simp]
 theorem εClosure'_split {update state stack' state₁ state₂} (hmem : state ∉ next) (hn : nfa[state] = .split state₁ state₂) :
-  εClosure' nfa wf pos next matched updates ((update, state) :: stack') = εClosure' nfa wf pos (next.insert state) matched updates ((update, state₁) :: (update, state₂) :: stack') := by
+  εClosure' nfa wf it next matched updates ((update, state) :: stack') = εClosure' nfa wf it (next.insert state) matched updates ((update, state₁) :: (update, state₂) :: stack') := by
   conv =>
     lhs
     unfold εClosure'
@@ -150,7 +150,7 @@ theorem εClosure'_split {update state stack' state₁ state₂} (hmem : state �
 
 @[simp]
 theorem εClosure'_save {update state stack' offset state'} (hmem : state ∉ next) (hn : nfa[state] = .save offset state') :
-  εClosure' nfa wf pos next matched updates ((update, state) :: stack') = εClosure' nfa wf pos (next.insert state) matched updates ((update ++ [(offset, pos)], state') :: stack') := by
+  εClosure' nfa wf it next matched updates ((update, state) :: stack') = εClosure' nfa wf it (next.insert state) matched updates ((update ++ [(offset, it.pos)], state') :: stack') := by
   conv =>
     lhs
     unfold εClosure'
@@ -159,7 +159,7 @@ theorem εClosure'_save {update state stack' offset state'} (hmem : state ∉ ne
 
 @[simp]
 theorem εClosure'_done {update state stack'} (hmem : state ∉ next) (hn : nfa[state] = .done) :
-  εClosure' nfa wf pos next matched updates ((update, state) :: stack') = εClosure' nfa wf pos (next.insert state) (matched <|> some update) (updates.set state state.isLt update) stack' := by
+  εClosure' nfa wf it next matched updates ((update, state) :: stack') = εClosure' nfa wf it (next.insert state) (matched <|> some update) (updates.set state state.isLt update) stack' := by
   conv =>
     lhs
     unfold εClosure'
@@ -168,7 +168,7 @@ theorem εClosure'_done {update state stack'} (hmem : state ∉ next) (hn : nfa[
 
 @[simp]
 theorem εClosure'_char {update state stack' c state'} (hmem : state ∉ next) (hn : nfa[state] = .char c state') :
-  εClosure' nfa wf pos next matched updates ((update, state) :: stack') = εClosure' nfa wf pos (next.insert state) matched (updates.set state state.isLt update) stack' := by
+  εClosure' nfa wf it next matched updates ((update, state) :: stack') = εClosure' nfa wf it (next.insert state) matched (updates.set state state.isLt update) stack' := by
   conv =>
     lhs
     unfold εClosure'
@@ -177,7 +177,7 @@ theorem εClosure'_char {update state stack' c state'} (hmem : state ∉ next) (
 
 @[simp]
 theorem εClosure'_sparse {update state stack' cs state'} (hmem : state ∉ next) (hn : nfa[state] = .sparse cs state') :
-  εClosure' nfa wf pos next matched updates ((update, state) :: stack') = εClosure' nfa wf pos (next.insert state) matched (updates.set state state.isLt update) stack' := by
+  εClosure' nfa wf it next matched updates ((update, state) :: stack') = εClosure' nfa wf it (next.insert state) matched (updates.set state state.isLt update) stack' := by
   conv =>
     lhs
     unfold εClosure'
@@ -186,7 +186,7 @@ theorem εClosure'_sparse {update state stack' cs state'} (hmem : state ∉ next
 
 @[simp]
 theorem εClosure'_fail {update state stack'} (hmem : state ∉ next) (hn : nfa[state] = .fail) :
-  εClosure' nfa wf pos next matched updates ((update, state) :: stack') = εClosure' nfa wf pos (next.insert state) matched updates stack' := by
+  εClosure' nfa wf it next matched updates ((update, state) :: stack') = εClosure' nfa wf it (next.insert state) matched updates stack' := by
   conv =>
     lhs
     unfold εClosure'
